Add print/read as primitives

src/client.hs
@@ -1,0 +1,11 @@
+module Client where
+
+import Network
+import System.IO 
+
+sendMessage msg = withSocketsDo $ do 
+        hSetBuffering stdout NoBuffering 
+        h <- connectTo "127.0.0.1" (PortNumber 8001)
+        hSetBuffering h LineBuffering
+        hPutStrLn h msg
+        hClose h
