src/server.hs
@@ -1,0 +1,42 @@
+import Network
+import System.IO 
+import Control.Exception
+import Handshake
+import Crypto.Saltine.Core.Box
+import Crypto.Saltine.Class
+import qualified Data.ByteString as BS
+
+main :: IO ()
+main = withSocketsDo $ do 
+    hSetBuffering stdout NoBuffering
+    server
+    putStrLn "Connection closed."
+
+coerce :: BS.ByteString -> [Integer]
+coerce = map toInteger . BS.unpack
+
+server :: IO ()
+server = do
+    sock <- listenOn (PortNumber 8001)
+    (pk,sk) <- newKeypair
+    core sock $ Left (((),coerce (encode pk)), coerce (encode sk))
+    sClose sock
+
+receive :: Socket -> IO Int
+receive sock = do
+    (h,host,port) <- accept sock
+    hSetBuffering h LineBuffering
+    msg <- hGetLine h           
+    putStrLn $ "received: " ++ msg
+    return $ read msg
+
+core sock x = 
+  case handshake_step x of
+    Nothing -> putStrLn "End"
+    Just (ExistT _ (e,next)) ->
+      case e of
+        GetE () -> receive sock >>= \n -> core sock (next $ unsafeCoerce n)
+        PutE n -> putStrLn (show n) >> core sock (next $ unsafeCoerce ())
+        ReadE () -> receive sock >>= \l -> core sock (next $ unsafeCoerce l)
+        PrintE l -> putStrLn (show l) >> core sock (next $ unsafeCoerce ())
+        GenKeyE _ -> newKeypair >>= \(sk,pk) -> core sock (next $ unsafeCoerce (coerce (encode sk) :: [Integer], coerce (encode pk) :: [Integer]))
